@@ -23,7 +23,7 @@ open Std (ExtTreeSet)
 
 section
 variable {hlc : HasLC} {GF : BundledGFunctors} [MachGS hlc GF] [CtokG GF] [UexecSG GF] [UprogSG GF]
-  [GhostMapG GF Nat (BitVec 8) RegMapF] [GhostVarG GF Nat] [GhostMapG GF Nat FdState RegMapF]
+  [GhostMapG GF Nat (BitVec 8) RegMapF] [GhostVarG GF Nat] [GhostMapG GF (Option Nat) UfdCell UfdMapF]
   [GhostVarG GF (ExtTreeSet GName compare)] [GhostVarG GF Int]
 
 /-- **Rocq `wp_kecho_strlen`**. -/
@@ -42,7 +42,7 @@ end
 /-- The interface of echo's `strlen`. -/
 structure ECHO_STRLEN : Prop where
   wp_echoStrlen : ∀ {hlc : HasLC} {GF : BundledGFunctors} [MachGS hlc GF] [CtokG GF] [UexecSG GF] [UprogSG GF]
-    [GhostMapG GF Nat (BitVec 8) RegMapF] [GhostVarG GF Nat] [GhostMapG GF Nat FdState RegMapF]
+    [GhostMapG GF Nat (BitVec 8) RegMapF] [GhostVarG GF Nat] [GhostMapG GF (Option Nat) UfdCell UfdMapF]
     [GhostVarG GF (ExtTreeSet GName compare)] [GhostVarG GF Int], wpEchoStrlenBody (hlc := hlc) (GF := GF)
 
 end Xv6
